Lean4Lean/Theory.lean
@@ -1,4 +1,5 @@
 import Lean4Lean.Theory.Typing.EnvLemmas
+import Lean4Lean.Theory.Typing.InductiveCertificate
 import Lean4Lean.Theory.Typing.Strong
 import Lean4Lean.Theory.Typing.UniqueTyping
 import Lean4Lean.Theory.Typing.ChurchRosser
